rename StaticMutrec* => Mutrec*

demo/mutrec/MutrecB.v
@@ -1,23 +1,94 @@
-Require Import List ZArith.
-Require Import CoqlibC Integers Floats AST Cop Asm.
-Require Import MutrecHeader.
+Require Import AST Coqlib.
+Require Import Asm.
+Require Import sflib.
+Require Import AsmC Mod.
+Require Import MutrecHeader Integers.
 
-Set Implicit Arguments.
+Definition _memoized : ident := 60%positive.
+Definition lb0: label := 1%positive.
+Definition lb1: label := 2%positive.
+Definition lb2: label := 3%positive.
 
-Local Open Scope Z_scope.
+Definition v_memoized := {|
+  gvar_info := tt;
+  gvar_init := (Init_int32 (Int.zero) :: Init_int32 (Int.zero) :: nil);
+  gvar_readonly := false;
+  gvar_volatile := false
+|}.
 
-Definition func_g: function := (admit "").
+Definition code: list instruction :=
+ [
+   (* .cfi_startproc *)
+   Pallocframe 32 (Ptrofs.repr 24) Ptrofs.zero ;
+     (* subq    $24, %rsp *)
+     (* .cfi_adjust_cfa_offset    24 *)
+     (* leaq    32(%rsp), %rax *)
+     (* movq    %rax, 0(%rsp) *)
+     Pmov_mr_a (Addrmode (Some RSP) None (inl 8)) RBX;
+     (* movq    %rbx, 8(%rsp) *)
+
+     Pmov_rr RBX RDI ;
+     (* movq    %rdi, %rbx *)
+     Ptestl_rr RBX RBX ;
+     (* testl    %ebx, %ebx *)
+     Pjcc Cond_ne lb0;
+     (* jne    .L100 *)
+     Pxorl_r RAX;
+     (* xorl    %eax, %eax *)
+     Pjmp_l lb1;
+     (* jmp    .L101 *)
+
+     Plabel lb0 ;
+     (* .L100: *)
+     Pmovl_rm RAX (Addrmode None None (inr (_memoized, Ptrofs.zero)));
+     (* movl	memoized(%rip), %eax *)
+     Pcmpl_rr RBX RAX;
+     (* cmpl	%eax, %ebx *)
+     Pjcc Cond_e lb2;
+     (* je	.L102 *)
+     Pleal RDI (Addrmode (Some RBX) None (inl (- 1)));
+     (* leal    -1(%ebx), %edi *)
+
+     Pcall_s f_id (mksignature [Tint] (Some Tint) cc_default);
+     (* call    f *)
+
+     Pleal RAX (Addrmode (Some RAX) (Some (RBX, 1)) (inl 0));
+     (* leal    0(%eax,%ebx,1), %eax *)
+     Pmovl_mr (Addrmode None None (inr (_memoized, Ptrofs.zero))) RBX;
+     (*	movl	%ebx, memoized(%rip) *)
+     Pmovl_mr (Addrmode None None (inr (_memoized, Ptrofs.repr 4))) RAX;
+     (*	movl	%eax, (memoized + 4)(%rip) *)
+     Pjmp_l lb1;
+     (* jmp    .L101 *)
+
+     Plabel lb2 ;
+     (* .L102: *)
+     Pmovl_rm RAX (Addrmode None None (inr (_memoized, Ptrofs.repr 4)));
+     (* movl	(memoized + 4)(%rip), %eax *)
+
+     Plabel lb1 ;
+     (* .L101: *)
+     Pmov_rm_a RBX (Addrmode (Some RSP) None (inl 8));
+     (* movq    8(%rsp), %rbx *)
+     Pfreeframe 32 (Ptrofs.repr 24) Ptrofs.zero;
+     (* addq    $24, %rsp *)
+     Pret
+       (* ret *)
+ ].
+
+Definition func_g: function :=
+  mkfunction (mksignature [Tint] (Some Tint) cc_default) code
+.
 
 Definition global_definitions : list (ident * globdef fundef unit) :=
 ((f_id,
    Gfun(External (EF_external "f"
-                   (mksignature (AST.Tint :: nil) (Some AST.Tint) cc_default))))
-   :: (g_id, Gfun(Internal func_g)) :: nil).
+                   (mksignature (AST.Tint :: nil) (Some AST.Tint) cc_default)))) :: (_memoized, Gvar v_memoized) ::
+ (g_id, Gfun(Internal func_g)) :: nil).
 
 Definition public_idents : list ident :=
 (f_id :: g_id :: nil).
 
-Definition prog : Asm.program := 
-  mkprogram global_definitions public_idents main_id.
+Definition prog: program := mkprogram global_definitions public_idents main_id.
 
-
+Definition md: Mod.t := AsmC.module prog.
