demo/mutrec/MutrecABspec.v
@@ -35,7 +35,7 @@ Section MODSEM.
       (i: int)
       (m: mem)
   | Returnstate
-      (i: int)
+      (s: int)
       (m: mem)
   .
 
@@ -52,6 +52,7 @@ Section MODSEM.
       (FINDF: Genv.find_funct ge args.(Args.fptr) = Some (AST.Internal func_fg))
       (VS: args.(Args.vs) = [Vint i])
       (M: args.(Args.m) = m)
+      (RANGE: 0 <= i.(Int.intval) < MAX)
     :
       initial_frame args (Callstate i m)
   .
@@ -65,9 +66,9 @@ Section MODSEM.
 
   Inductive final_frame: state -> Retv.t -> Prop :=
   | final_frame_return
-      i m
+      s m
     :
-      final_frame (Returnstate i m) (Retv.mk (Vint i) m)
+      final_frame (Returnstate s m) (Retv.mk (Vint s) m)
   .
 
   Program Definition modsem: ModSem.t :=
@@ -79,7 +80,7 @@ Section MODSEM.
       ModSem.after_external := bot3;
       ModSem.globalenv := ge;
       ModSem.skenv := skenv;
-      ModSem.skenv_link := skenv_link; 
+      ModSem.skenv_link := skenv_link;
     |}
   .
 
